feature: memories store labeled values rather than ownership

src/Memory/Memory_func.v
@@ -3,16 +3,16 @@ Require Import SpecCert.Memory.Memory_def.
 Require Import SpecCert.Map.
 
 Definition find_in_memory
-           {S   :Set}
-           (mem :Memory S)
-           (ha  :HardwareAddress)
+           {S:   Type}
+           (mem: Memory S)
+           (ha:  HardwareAddress)
            :S :=
   find_in_map mem ha.
 
 Definition update_in_memory
-           {S      :Set}
-           (mem    :Memory S)
-           (ha     :HardwareAddress)
-           (owner :S)
+           {S:      Type}
+           (mem:    Memory S)
+           (ha:     HardwareAddress)
+           (value:  S)
            :Memory S :=
-  add_in_map mem ha owner.
+  add_in_map mem ha value.
