src/x86/Transition/Event/Read.v
@@ -1,11 +1,19 @@
 Require Import SpecCert.x86.Architecture.
+Require Import SpecCert.x86.Value.
 Require Import SpecCert.Address.
 Require Import SpecCert.Cache.
 Require Import SpecCert.Interval.
 
+Definition read_pre
+           {Label: Type}
+           (pa:    PhysicalAddress)
+           (val:   Value)
+           (a:     Architecture Label) :=
+  option_map fst (find_address_content a pa) = Some val.
+
 Definition read_uncachable_post
-           {S :Set}
-           (a :Architecture S)
+           {Label: Type}
+           (a:     Architecture Label)
            (pa:PhysicalAddress) :=
   a.
 
@@ -13,32 +21,25 @@ Definition read_uncachable_post
    "If the logical processor is not in SMM, (...) read
    access return a fixed value for each byte" *)
 Definition read_smrrhit_post
-           {S  :Set}
-           (a  :Architecture S)
-           (pa :PhysicalAddress) :=
+           {Label: Type}
+           (a:     Architecture Label)
+           (pa:    PhysicalAddress) :=
   a.
 
 Definition read_writeback_post
-           {S  :Set}
-           (a  :Architecture S)
-           (pa :PhysicalAddress) :=
+           {Label: Type}
+           (a:     Architecture Label)
+           (pa:    PhysicalAddress) :=
   if cache_hit_dec (cache a) pa
   then a
   else load_in_cache_from_memory a pa.
 
 Definition read_post
-           {S  :Set}
-           (pa :PhysicalAddress) :=
-  fun (a a':Architecture S) =>
+           {Label: Type}
+           (pa:    PhysicalAddress) :=
+  fun (a a':Architecture Label) =>
     match resolve_cache_strategy (proc a) pa with
     | Uncachable => a' = read_uncachable_post a pa
     | WriteBack  => a' = read_writeback_post a pa
     | SmrrHit    => a' = read_smrrhit_post a pa
     end.
-
-(*
-Definition exec_pre
-           {S :Type} :=
-  fun (a :Architecture S) =>
-    find_address_content a (ip (proc a)) = Some (context a).
-*)
