src/x86/Transition/Transition_def.v
@@ -5,45 +5,45 @@ Require Import SpecCert.x86.Architecture.
 Require Import SpecCert.x86.Transition.Event.
 
 Definition x86Context
-           (S: Set)
-  := HardwareSoftwareMapping (Architecture S) S.
+           (S: Type) :=
+  HardwareSoftwareMapping (Architecture S) S.
 
 Definition pre_condition
-           {S :Set} :=
+           {S :Type} :=
   Architecture S -> Prop.
 
 Definition post_condition
-           {S :Set} :=
+           {S :Type} :=
   Architecture S -> Architecture S -> Prop.
 
 Definition no_pre
-           {S :Set} :=
+           {S :Type} :=
   fun (a: Architecture S) => True.
 
 Definition id_post
-           {S :Set} :=
+           {S :Type} :=
   fun (a a':Architecture S) => a = a'.
 
 Definition x86_precondition
-           {S:  Set}
-           (h:  Architecture S)
+           {Label: Type}
+           (a:  Architecture Label)
            (ev: x86Event)
   : Prop :=
   match ev with
   | software DisableInterrupt     => no_pre
   | software EnableInterrupt      => no_pre
   | software (Write addr value)   => no_pre
-  | software (Read addr value)    => no_pre
+  | software (Read addr value)    => read_pre addr value
   | software OpenSmram            => open_smram_pre
   | software CloseSmram           => close_smram_pre
   | software LockSmramc           => lock_smramc_pre
   | software (NextInstruction pa) => no_pre
   | hardware (ReceiveInterrupt i) => no_pre
-  | hardware (Exec value)         => no_pre
-  end h.
+  | hardware (Exec value)         => read_pre (ip (proc a)) value
+  end a.
 
 Definition x86_postcondition
-           {S:       Set}
+           {S:       Type}
            (context: x86Context S)
            (h:       Architecture S)
            (ev:      x86Event)
@@ -52,7 +52,7 @@ Definition x86_postcondition
   match ev with
   | software DisableInterrupt     => disable_interrupt_post
   | software EnableInterrupt      => enable_interrupt_post
-  | software (Write addr value)   => write_post context addr
+  | software (Write addr value)   => write_post context addr value
   | software (Read addr value)    => read_post addr
   | software OpenSmram            => open_smram_post
   | software CloseSmram           => close_smram_post
