src/Memory/Memory_def.v
@@ -1,4 +1,4 @@
 Require Import SpecCert.Address.
 Require Import SpecCert.Map.
 
-Definition Memory (S:Set) := Map HardwareAddress S.
+Definition Memory (S: Type) := Map HardwareAddress S.
