src/Smm/Delta/Preserve/Architecture.v
@@ -62,53 +62,59 @@ Proof.
     * apply eq_refl.
 Qed.
 
-Lemma update_memory_content_with_cache_content_preserves_smram_code_inv:
-  forall a a' :Architecture Software,
-  forall pa   :PhysicalAddress,
-    inv a
-    -> a' = update_memory_content a
-                                 (phys_to_hard a (cache_location_address (cache a) pa))
-                                 (find_in_cache_location (cache a) pa)
-    -> smram_code_inv a'.
+Lemma update_memory_content_with_cache_content_preserves_smram_code_inv
+      (a a': Architecture Software)
+      (pa:   PhysicalAddress)
+  : let cont := find_in_cache_location (cache a) pa
+    in inv a
+       -> a' = update_memory_content a
+                                     (phys_to_hard a (cache_location_address (cache a) pa))
+                                     cont
+       -> smram_code_inv a'.
 Proof.
-  intros a a' pa.
+  simpl.
   remember (cache_location_address (cache a) pa) as pa'.
   remember (find_in_cache_location (cache a) pa) as c'.
   remember (phys_to_hard a pa') as ha.
   intros [Hsmramc [Hsmram [Hsmrr [Hclean [Hip Hsmbase]]]]] Heqa'.
   destruct (is_inside_smram_dec pa') as [Hinside|Houtside].
   + rewrite (cache_location_cache_location (cache a) pa pa') in Heqc'; [
-    | apply hardware_ensures_cache_is_well_formed
+    | apply x86_cache_is_well_formed
     | trivial
     ].
     symmetry in Heqc'.
     apply find_in_cache_cache_location in Heqc'; [
-      | apply hardware_ensures_cache_is_well_formed ].
+      | apply x86_cache_is_well_formed ].
     assert (cache_hit (cache a) pa') as Hhit.
     rewrite Heqpa';
       apply cache_hit_cache_location_address;
-      apply hardware_ensures_cache_is_well_formed.
+      apply x86_cache_is_well_formed.
     rewrite <- cache_hit_cache_location_cache_find in Heqc'; [
       | trivial
       ].
     unfold cache_clean_inv in *.
     unfold find_cache_content in Hclean.
-    rewrite Hclean in Heqc'; try trivial.
+    induction c' as [v s].
+    assert (s = smm).
+    apply (Hclean pa' v s Hinside Hhit Heqc').
     unfold smram_code_inv.
-    intros addr Haddr.
-    induction c'; [| inversion Heqc' ].
-    rewrite Heqa'.
-    destruct (eq_dec ha (dram addr)) as [Heq|_H].
+    intros addr val s' Hinside' Hfind.
+    rewrite H in Heqa'.
+    destruct (eq_dec ha (dram addr)) as [Heq|Hneq].
     * apply eq_equal in Heq.
-      rewrite Heq.
-      rewrite update_ha_in_memory_is_ha.
-      trivial.
-    * rewrite <- (update_ha_in_memory_changes_only_ha a ha (dram addr) smm); [
-      | trivial
-      ].
-      apply Hsmram; trivial.
+      rewrite Heqa' in Hfind.
+      rewrite Heq in Hfind.
+      rewrite update_ha_in_memory_is_ha in Hfind.
+      inversion Hfind.
+      reflexivity.
+    * rewrite Heqa' in Hfind.
+      unfold find_memory_content, find_in_memory, update_memory_content, update_in_memory in Hfind.
+      simpl in Hfind.
+      rewrite <- add_2 in Hfind; [| exact Hneq].
+      unfold smram_code_inv in Hsmram.
+      apply (Hsmram addr val s' Hinside' Hfind).
   + unfold smram_code_inv.
-    intros addr Haddr.
+    intros addr val s Haddr.
     unfold phys_to_hard, translate_physical_address in Heqha.
     destruct (is_inside_smram_dec pa') as [_H|_H']; [ intuition |].
     rewrite Heqha in *.
@@ -127,20 +133,19 @@ Proof.
       trivial.
 Qed.
 
-Lemma update_memory_content_with_cache_content_preserves_cache_clean_inv:
-  forall a a' :Architecture Software,
-  forall pa   :PhysicalAddress,
-    inv a
-    -> a' = update_memory_content a
-                                 (phys_to_hard a (cache_location_address (cache a) pa))
-                                 (find_in_cache_location (cache a) pa)
-    -> cache_clean_inv a'.
+Lemma update_memory_content_with_cache_content_preserves_cache_clean_inv
+      (a a':  Architecture Software)
+      (pa:    PhysicalAddress)
+      (Hinv:  inv a)
+      (Heqa': a' = update_memory_content a
+                                         (phys_to_hard a (cache_location_address (cache a) pa))
+                                         (find_in_cache_location (cache a) pa))
+  : cache_clean_inv a'.
 Proof.
-  intros a a' pa.
   remember (cache_location_address (cache a) pa) as pa'.
   remember (find_in_cache_location (cache a) pa) as c'.
   remember (phys_to_hard a pa') as ha'.
-  intros [Hsmramc [Hsmram [Hsmrr [Hclean [Hip Hsmbase]]]]] Heqa'.
+  destruct Hinv as [Hsmramc [Hsmram [Hsmrr [Hclean [Hip Hsmbase]]]]].
   unfold cache_clean_inv.
   unfold find_cache_content.
   apply update_memory_changes_only_memory in Heqa'.
@@ -266,53 +271,56 @@ Proof.
     | eapply (update_memory_content_with_cache_content_preserves_smbase_inv a a' pa) ]; trivial.
 Qed.
 
-Lemma update_memory_content_with_context_preserves_smram_code_inv:
-  forall a a' :Architecture Software,
-  forall pa   :PhysicalAddress,
-    inv a
-    -> a' = update_memory_content a (phys_to_hard a pa) (smm_context a)
-    -> smram_code_inv a'.
+Lemma update_memory_content_with_context_preserves_smram_code_inv
+      (a a':   Architecture Software)
+      (pa:     PhysicalAddress)
+      (val:    Value)
+      (Hinv:   inv a)
+      (Heqa': a' = update_memory_content a (phys_to_hard a pa) (val, smm_context a))
+    : smram_code_inv a'.
 Proof.
-  intros a a' pa [Hsmramc [Hsmram [Hclean [Hsmrr [Hip Hsmbase]]]]] Heqa'.
+  destruct Hinv as [Hsmramc [Hsmram [Hclean [Hsmrr [Hip Hsmbase]]]]].
   unfold smram_code_inv.
-  intros pa' Hinside'.
+  intros pa' val' s Hinside' Hfind.
   unfold update_memory_content in Heqa'.
   unfold update_in_memory in Heqa'.
   unfold find_memory_content, find_in_memory.
-  rewrite Heqa'.
-  simpl.
-  unfold phys_to_hard, translate_physical_address.
+  rewrite Heqa' in Hfind.
+  unfold find_memory_content, find_in_memory in Hfind.
+  simpl in Hfind.
+  unfold phys_to_hard, translate_physical_address in Hfind.
   destruct is_inside_smram_dec as [Hinside|Houtside].
-  + destruct can_access_smram_dec.
-    * assert (smm_context a = smm).
-      unfold can_access_smram in c.
-      destruct c as [Hsmm|Hfalse].
-      unfold smm_context.
-      destruct is_in_smm_dec; try reflexivity.
-      unfold is_in_smm in n.
-      apply n in Hsmm.
-      destruct Hsmm.
-      unfold smramc_inv in Hsmramc.
-      unfold smramc_is_locked in Hsmramc.
-      unfold smramc_is_ro in Hsmramc.
-      apply (lock_is_close (smramc (memory_controller a))) in Hsmramc.
-      rewrite Hsmramc in Hfalse.
-      discriminate.
-      rewrite H.
-      destruct (eq_dec pa pa').
-      apply eq_equal in e.
-      rewrite e.
-      apply add_1.
-      rewrite <- add_2.
-      apply Hsmram.
-      exact Hinside'.
-      intro Hfalse.
-      apply hardware_dram_cast in Hfalse.
-      apply n in Hfalse.
-      exact Hfalse.
-    * rewrite <- add_2.
-      apply Hsmram.
-      exact Hinside'.
+  + destruct can_access_smram_dec as [Hcan|Hcannot].
+    * assert (smm_context a = smm) as Hcontext.
+      - unfold can_access_smram in Hcan.
+        destruct Hcan as [Hsmm|Hfalse].
+        unfold smm_context.
+        destruct is_in_smm_dec as [Hin|Hnotin]; try reflexivity.
+        unfold is_in_smm in Hnotin.
+        apply Hnotin in Hsmm.
+        destruct Hsmm.
+        unfold smramc_inv in Hsmramc.
+        unfold smramc_is_locked in Hsmramc.
+        unfold smramc_is_ro in Hsmramc.
+        apply (lock_is_close (smramc (memory_controller a))) in Hsmramc.
+        rewrite Hsmramc in Hfalse.
+        discriminate.
+      - rewrite Hcontext in Hfind.
+        destruct (eq_dec pa pa').
+        apply eq_equal in e.
+        rewrite e in Hfind.
+        rewrite add_1 in Hfind.
+        inversion Hfind.
+        reflexivity.
+        rewrite <- add_2 in Hfind.
+        unfold smram_code_inv in Hsmram.
+        apply (Hsmram pa' val' s Hinside' Hfind).
+        intro Hfalse.
+        apply hardware_dram_cast in Hfalse.
+        apply n in Hfalse.
+        exact Hfalse.
+    * rewrite <- add_2 in Hfind.
+      apply (Hsmram pa' val' s Hinside' Hfind).
       intro H.
       apply eq_sym in H.
       assert (~ eq (dram pa') (vga pa)).
@@ -321,49 +329,53 @@ Proof.
       exact H.
   + assert (~ eq pa pa') as Hneqpapa'.
     apply (pa1_not_in_interval_pa2_in_interval_pa1_neq_pa2 pa pa' smram_space Houtside Hinside').
-    rewrite <- (add_2 (memory a) (dram pa) (dram pa')); [ apply Hsmram; apply Hinside'|].
-    intro Hfalse.
-    apply hardware_dram_cast in Hfalse.
-    apply Hneqpapa' in Hfalse.
-    exact Hfalse.
+    rewrite <- (add_2 (memory a) (dram pa) (dram pa')) in Hfind.
+    * apply (Hsmram pa' val' s Hinside' Hfind).
+    * intro Hfalse.
+      apply hardware_dram_cast in Hfalse.
+      apply Hneqpapa' in Hfalse.
+      exact Hfalse.
 Qed.
 
-Lemma update_memory_content_with_context_preserves_smramc_inv:
-  forall a a' :Architecture Software,
-  forall pa   :PhysicalAddress,
-    inv a
-    -> a' = update_memory_content a (phys_to_hard a pa) (smm_context a)
-    -> smramc_inv a'.
+Lemma update_memory_content_with_context_preserves_smramc_inv
+      (a a':  Architecture Software)
+      (pa:    PhysicalAddress)
+      (val:   Value)
+      (Hinv:  inv a)
+      (Heqa': a' = update_memory_content a (phys_to_hard a pa) (val, smm_context a))
+  : smramc_inv a'.
 Proof.
-  intros a a' pa [Hsmramc [Hsmram [Hsmrr [Hclean [Hip Hsmbase]]]]] Heqa'.
+  destruct Hinv as [Hsmramc [Hsmram [Hsmrr [Hclean [Hip Hsmbase]]]]].
   apply update_memory_changes_only_memory in Heqa' as [Hmc [Hproc Hother]].
   unfold smramc_inv.
   rewrite <- Hmc.
   exact Hsmramc.
 Qed.
 
-Lemma update_memory_content_with_context_preserves_smbase_inv:
-  forall a a' :Architecture Software,
-  forall pa   :PhysicalAddress,
-    inv a
-    -> a' = update_memory_content a (phys_to_hard a pa) (smm_context a)
-    -> smbase_inv a'.
+Lemma update_memory_content_with_context_preserves_smbase_inv
+      (a a':  Architecture Software)
+      (pa:    PhysicalAddress)
+      (val:   Value)
+      (Hinv:  inv a)
+      (Heqa': a' = update_memory_content a (phys_to_hard a pa) (val, smm_context a))
+  : smbase_inv a'.
 Proof.
-  intros a a' pa [Hsmramc [Hsmram [Hsmrr [Hclean [Hip Hsmbase]]]]] Heqa'.
+  destruct Hinv as [Hsmramc [Hsmram [Hsmrr [Hclean [Hip Hsmbase]]]]].
   apply update_memory_changes_only_memory in Heqa' as [Hmc [Hproc Hother]].
   unfold smbase_inv.
   rewrite <- Hproc.
   exact Hsmbase.
 Qed.
 
-Lemma update_memory_content_with_context_preserves_cache_clean_inv:
-  forall a a' :Architecture Software,
-  forall pa   :PhysicalAddress,
-    inv a
-    -> a' = update_memory_content a (phys_to_hard a pa) (smm_context a)
-    -> cache_clean_inv a'.
+Lemma update_memory_content_with_context_preserves_cache_clean_inv
+      (a a':  Architecture Software)
+      (pa:    PhysicalAddress)
+      (val:   Value)
+      (Hinv:  inv a)
+      (Heqa': a' = update_memory_content a (phys_to_hard a pa) (val, smm_context a))
+  : cache_clean_inv a'.
 Proof.
-  intros a a' pa [Hsmramc [Hsmram [Hsmrr [Hclean Hip]]]] Heqa'.
+  destruct Hinv as [Hsmramc [Hsmram [Hsmrr [Hclean Hip]]]].
   apply update_memory_changes_only_memory in Heqa' as [Hmc [Hproc Hother]].
   unfold cache_clean_inv.
   unfold find_cache_content.
@@ -371,28 +383,30 @@ Proof.
   exact Hclean.
 Qed.
 
-Lemma update_memory_content_with_context_preserves_smrr_inv:
-  forall a a' :Architecture Software,
-  forall pa   :PhysicalAddress,
-    inv a
-    -> a' = update_memory_content a (phys_to_hard a pa) (smm_context a)
-    -> smrr_inv a'.
+Lemma update_memory_content_with_context_preserves_smrr_inv
+      (a a':  Architecture Software)
+      (pa:    PhysicalAddress)
+      (val:   Value)
+      (Hinv:  inv a)
+      (Heqa': a' = update_memory_content a (phys_to_hard a pa) (val, smm_context a))
+  : smrr_inv a'.
 Proof.
-  intros a a' pa [Hsmramc [Hsmram [Hsmrr [Hclean Hip]]]] Heqa'.
+  destruct Hinv as [Hsmramc [Hsmram [Hsmrr [Hclean Hip]]]].
   apply update_memory_changes_only_memory in Heqa' as [Hmc [Hproc Hother]].
   unfold smrr_inv.
   rewrite <- Hproc.
   exact Hsmrr.
 Qed.
 
-Lemma update_memory_content_with_context_preserves_ip_inv:
-  forall a a' :Architecture Software,
-  forall pa   :PhysicalAddress,
-    inv a
-    -> a' = update_memory_content a (phys_to_hard a pa) (smm_context a)
-    -> ip_inv a'.
+Lemma update_memory_content_with_context_preserves_ip_inv
+      (a a':  Architecture Software)
+      (pa:    PhysicalAddress)
+      (val:   Value)
+      (Hinv:  inv a)
+      (Heqa': a' = update_memory_content a (phys_to_hard a pa) (val, smm_context a))
+  : ip_inv a'.
 Proof.
-  intros a a' pa [Hsmramc [Hsmram [Hsmrr [Hclean [Hip Hsmbase]]]]] Heqa'.
+  destruct Hinv as [Hsmramc [Hsmram [Hsmrr [Hclean [Hip Hsmbase]]]]].
   apply update_memory_changes_only_memory in Heqa' as [Hmc [Hproc Hother]].
   unfold ip_inv.
   rewrite <- Hproc.
@@ -400,33 +414,32 @@ Proof.
   exact Hip.
 Qed.
 
-Lemma update_memory_content_with_context_preserves_inv:
-  forall a a' :Architecture Software,
-  forall pa   :PhysicalAddress,
-    inv a
-    -> a' = update_memory_content a (phys_to_hard a pa) (smm_context a)
-    -> inv a'.
+Lemma update_memory_content_with_context_preserves_inv
+      (a a':  Architecture Software)
+      (pa:    PhysicalAddress)
+      (val:   Value)
+      (Hinv:  inv a)
+      (Heqa': a' = update_memory_content a (phys_to_hard a pa) (val, smm_context a))
+  : inv a'.
 Proof.
-  intros a a' pa.
-  intros Hinv Heqa'.
   unfold inv.
   split; [| split; [| split; [| split; [| split]]]]; [
-      eapply (update_memory_content_with_context_preserves_smramc_inv a a' pa)
-    | eapply (update_memory_content_with_context_preserves_smram_code_inv a a' pa)
-    | eapply (update_memory_content_with_context_preserves_smrr_inv a a' pa)
-    | eapply (update_memory_content_with_context_preserves_cache_clean_inv a a' pa)
-    | eapply (update_memory_content_with_context_preserves_ip_inv a a' pa)
-    | eapply (update_memory_content_with_context_preserves_smbase_inv a a' pa) ]; trivial.
+      eapply (update_memory_content_with_context_preserves_smramc_inv a a' pa val)
+    | eapply (update_memory_content_with_context_preserves_smram_code_inv a a' pa val)
+    | eapply (update_memory_content_with_context_preserves_smrr_inv a a' pa val)
+    | eapply (update_memory_content_with_context_preserves_cache_clean_inv a a' pa val)
+    | eapply (update_memory_content_with_context_preserves_ip_inv a a' pa val)
+    | eapply (update_memory_content_with_context_preserves_smbase_inv a a' pa val) ]; trivial.
 Qed.
 
-Lemma load_in_cache_from_memory_preserves_smram_code_inv:
-  forall a a' :Architecture Software,
-  forall pa   :PhysicalAddress,
-    inv a
-    -> a' = load_in_cache_from_memory a pa
-    -> smram_code_inv a'.
+Lemma load_in_cache_from_memory_preserves_smram_code_inv
+      (a a':    Architecture Software)
+      (pa:      PhysicalAddress)
+      (Hinv:    inv a)
+      (Heqa':   a' = load_in_cache_from_memory a pa)
+  : smram_code_inv a'.
 Proof.
-  intros a a' pa [Hsmramc [Hsmram [Hsmrr [Hclean [Hip Hsmbase]]]]] Heqa'.
+  destruct Hinv as [Hsmramc [Hsmram [Hsmrr [Hclean [Hip Hsmbase]]]]].
   assert (inv a) as Hinv.
   split; [ exact Hsmramc
          | split; [ exact Hsmram
@@ -454,14 +467,177 @@ Proof.
     exact Hsmram.
 Qed.
 
-Lemma load_in_cache_from_memory_preserves_cache_clean_inv:
-  forall a a' :Architecture Software,
-  forall pa   :PhysicalAddress,
-    inv a -> (is_inside_smram pa -> is_in_smm (proc a))
-    -> a' = load_in_cache_from_memory a pa
-    -> cache_clean_inv a'.
+Lemma update_cache_with_memory_cache_clean_inv
+      (a a':  Architecture Software)
+      (pa:    PhysicalAddress)
+      (Hinv:  inv a)
+      (Hin_smm: (is_inside_smram pa -> is_in_smm (proc a)))
+      (Heqa': a' = update_cache_content a pa (find_memory_content a (phys_to_hard a pa)))
+  : cache_clean_inv a'.
 Proof.
-  intros a a' pa [Hsmramc [Hsmram [Hsmrr [Hclean [Hip Hsmbase]]]]] Hin_smm Heqa'.
+  destruct Hinv as [Hsmramc [Hsmram [Hsmrr [Hclean [Hip Hsmbase]]]]].
+  unfold cache_clean_inv, find_cache_content.
+  intros pa' v' s Hinside' Hcache_hit Hfind.
+  remember (find_memory_content a (phys_to_hard a pa)) as c'.
+  unfold update_cache_content in Heqa'.
+  rewrite Heqa' in Hfind.
+  simpl in Hfind.
+  unfold global_update_in_cache in Hfind.
+  destruct (cache_hit_dec (cache a) pa) as [Hcache_hit_pa|Hnot_cache_hit_pa].
+  * unfold update_in_cache, find_in_cache in Hfind.
+    destruct (eq_dec pa pa') as [Heqpapa'|Hneqpapa'].
+    - apply eq_equal in Heqpapa'.
+      rewrite Heqpapa' in Hfind.
+      assert (cache_hit
+                (add_in_map (cache a) (phys_to_index pa')
+                            {| dirty := true; content := c'; tag := pa' |}) pa') as Hcache_hit_add.
+      unfold cache_hit.
+      rewrite add_1.
+      apply eq_refl.
+      destruct (cache_hit_dec
+                (add_in_map (cache a) (phys_to_index pa')
+                            {| dirty := true; content := c'; tag := pa' |}) pa');
+        [| intuition].
+      rewrite add_1 in Hfind.
+      simpl in Hfind.
+      rewrite Heqpapa' in Heqc'.
+      unfold phys_to_hard, translate_physical_address in Heqc'.
+      destruct (is_inside_smram_dec pa') as [Hinside|_H]; [| intuition ].
+      assert (is_in_smm (proc a)); [
+          rewrite <- Heqpapa' in Hinside;
+          apply (Hin_smm Hinside) |].
+      destruct (can_access_smram_dec (memory_controller a) (in_smm (proc a))) as [Hcan|Hcannot]; [
+        |  unfold can_access_smram in Hcannot;
+          intuition ].
+      destruct c'.
+      apply (Hsmram pa' v s Hinside).
+      rewrite <- Heqc'.
+      inversion Hfind.
+      reflexivity.
+    - destruct (eq_dec (phys_to_index pa) (phys_to_index pa')) as [Heqi|Hneqi].
+      assert (cache_hit (cache a') pa); [
+          rewrite Heqa';
+          simpl;
+          apply global_update_in_cache_cache_hit |].
+      assert (~ cache_hit (cache a') pa'); [
+          apply (cache_hit_same_index_cache_miss (cache a') pa); trivial
+        | intuition ].
+      assert (cache_hit
+                (add_in_map (cache a) (phys_to_index pa)
+                            {| dirty := true; content := c'; tag := pa |}) pa').
+      unfold cache_hit.
+      rewrite <- add_2; [| exact Hneqi ].
+      rewrite Heqa' in Hcache_hit.
+      simpl in Hcache_hit.
+      unfold cache_hit, global_update_in_cache in Hcache_hit.
+      destruct (cache_hit_dec (cache a) pa) as [Hcache_hit_x_pa|Hncache_hit_x_pa].
+      unfold update_in_cache in Hcache_hit.
+      rewrite <- add_2 in Hcache_hit; [| exact Hneqi ].
+      exact Hcache_hit.
+      apply Hncache_hit_x_pa in Hcache_hit_pa.
+      destruct Hcache_hit_pa.
+      destruct (cache_hit_dec
+                  (add_in_map (cache a) (phys_to_index pa)
+                              {| dirty := true; content := c'; tag := pa |}) pa') as [Hcache_add|Hncache_add].
+      rewrite <- add_2 in Hfind.
+      unfold cache_clean_inv in Hclean.
+      assert (cache_hit (cache a) pa') as Hcache_hit_x_pa'; [
+          apply (cache_hit_is_preserve_by_non_conflicted_update (cache a)
+                                                                (cache a')
+                                                                pa
+                                                                pa'
+                                                                c'); [
+          exact Hneqi |
+          rewrite Heqa'; simpl; reflexivity |
+          exact Hcache_hit ] |].
+      assert (find_cache_content a pa' = Some (content (find_in_map (cache a) (phys_to_index pa')))) as Hfind'.
+      unfold find_cache_content, find_in_cache.
+      destruct (cache_hit_dec (cache a) pa') as [_H|_H]; [ reflexivity | intuition ].
+      apply (Hclean pa' v' s Hinside' Hcache_hit_x_pa').
+      inversion Hfind.
+      exact Hfind'.
+      exact Hneqi.
+      discriminate Hfind.
+  * destruct (eq_dec (phys_to_index pa) (phys_to_index pa')) as [Heqi|Hneqi].
+    - assert (cache a'=global_update_in_cache (cache a) pa c') as Heqcache'; [
+        rewrite Heqa';
+        simpl;
+        reflexivity |].
+      assert (cache_hit (global_update_in_cache (cache a) pa c') pa); [
+          apply (global_update_in_cache_cache_hit (cache a) pa) |].
+      rewrite <- Heqcache' in H.
+      destruct (eq_dec pa pa') as [Heq|Hneq].
+      (* case addr_eq *)
+      apply eq_equal in Heq.
+      rewrite Heq in Heqc'.
+      unfold smram_code_inv in Hsmram.
+      assert (is_inside_smram pa'); try exact Hinside'.
+      rewrite <- Heq in Hinside'.
+      apply Hin_smm in Hinside'.
+      unfold is_in_smm in Hinside'.
+      unfold phys_to_hard, translate_physical_address in Heqc'.
+      rewrite <- Heq in Heqc'.
+      destruct (is_inside_smram_dec pa).
+      rewrite Hinside' in Heqc'.
+      destruct (can_access_smram_dec (memory_controller a) true).
+      destruct c' as [v l].
+      assert (l = smm).
+      apply (Hsmram pa v l i).
+      symmetry; exact Heqc'.
+      rewrite H1 in *.
+      unfold find_in_cache, load_in_cache in Hfind.
+      rewrite <- Heq in Hfind.
+      destruct cache_hit_dec.
+      rewrite add_1 in Hfind.
+      simpl in Hfind.
+      inversion Hfind.
+      reflexivity.
+      unfold cache_hit in n.
+      rewrite add_1 in n.
+      simpl in n.
+      unfold not in n.
+      assert (eq pa pa) by (apply eq_refl).
+      apply n in H2.
+      destruct H2.
+      unfold can_access_smram in n.
+      apply not_or_and in n.
+      destruct n as [G1 G2].
+      intuition.
+      rewrite <- Heq in H0.
+      intuition.
+      (* case ~ addr_eq *)
+      apply (global_update_not_cache_hit (cache a) (cache a') pa pa' c') in Heqcache'; try intuition.
+    - unfold find_in_cache, load_in_cache in Hfind.
+      destruct cache_hit_dec.
+      rewrite <- add_2 in Hfind.
+      assert (cache_hit (cache a) pa') as Hcache_hit_before; [
+          apply (cache_hit_is_preserve_by_non_conflicted_update (cache a)
+                                                                (cache a')
+                                                                pa
+                                                                pa'
+                                                                c'); [
+            exact Hneqi
+          | rewrite Heqa'; reflexivity
+          | exact Hcache_hit ] |].
+      unfold cache_clean_inv in Hclean.
+      inversion Hfind.
+      apply (Hclean pa' v' s Hinside' Hcache_hit_before).
+      unfold find_cache_content.
+      unfold find_in_cache.
+      destruct cache_hit_dec; intuition.
+      exact Hneqi.
+      discriminate Hfind.
+Qed.
+
+Lemma load_in_cache_from_memory_preserves_cache_clean_inv
+      (a a':  Architecture Software)
+      (pa:    PhysicalAddress)
+      (Hinv:  inv a)
+      (Hin_smm: (is_inside_smram pa -> is_in_smm (proc a)))
+      (Heqa': a' = load_in_cache_from_memory a pa)
+  : cache_clean_inv a'.
+Proof.
+  destruct Hinv as [Hsmramc [Hsmram [Hsmrr [Hclean [Hip Hsmbase]]]]].
   assert (inv a) as Hinv.
   split; [ exact Hsmramc
          | split; [ exact Hsmram
@@ -474,427 +650,72 @@ Proof.
   + remember (update_memory_content a
                                     (phys_to_hard a (cache_location_address (cache a) pa))
                                     (find_in_cache_location (cache a) pa)) as ax.
-    assert (inv ax).
+    assert (inv ax) as Hinvx.
     apply (update_memory_content_with_cache_content_preserves_inv a ax pa); trivial.
-    unfold cache_clean_inv, find_cache_content.
-    intros pa' Hinside' Hcache_hit.
-    remember (find_memory_content a (phys_to_hard a pa)) as c'.
-    unfold update_cache_content in Heqa'.
-    rewrite Heqa'; simpl.
-    unfold global_update_in_cache.
-    destruct (cache_hit_dec (cache ax) pa) as [Hcache_hit_pa|Hnot_cache_hit_pa].
-    * unfold update_in_cache, find_in_cache.
-      destruct (eq_dec pa pa') as [Heqpapa'|Hneqpapa'].
-      - apply eq_equal in Heqpapa'.
-        rewrite Heqpapa'.
-        assert (cache_hit
-                  (add_in_map (cache ax) (phys_to_index pa')
-                              {| dirty := true; content := c'; tag := pa' |}) pa') as Hcache_hit_add.
-        unfold cache_hit.
-        rewrite add_1.
-        apply eq_refl.
-        destruct (cache_hit_dec
-                  (add_in_map (cache ax) (phys_to_index pa')
-                              {| dirty := true; content := c'; tag := pa' |}) pa');
-          [| intuition].
-        rewrite add_1.
-        simpl.
-        rewrite Heqpapa' in Heqc'.
-        unfold phys_to_hard, translate_physical_address in Heqc'.
-        destruct (is_inside_smram_dec pa') as [Hinside|_H]; [| intuition ].
-        assert (is_in_smm (proc a)); [
-            rewrite <- Heqpapa' in Hinside;
-            apply (Hin_smm Hinside) |].
-        destruct (can_access_smram_dec (memory_controller a) (in_smm (proc a))) as [Hcan|Hcannot]; [
-          |  unfold can_access_smram in Hcannot;
-            intuition ].
-        rewrite Hsmram in Heqc'; [| exact Hinside ].
-        rewrite Heqc'.
-        reflexivity.
-      - destruct (eq_dec (phys_to_index pa) (phys_to_index pa')) as [Heqi|Hneqi].
-        assert (cache_hit (cache a') pa); [
-            rewrite Heqa';
-            simpl;
-            apply global_update_in_cache_cache_hit |].
-        assert (~ cache_hit (cache a') pa'); [
-            apply (cache_hit_same_index_cache_miss (cache a') pa); trivial
-          | intuition ].
-        assert (cache_hit
-                  (add_in_map (cache ax) (phys_to_index pa)
-                              {| dirty := true; content := c'; tag := pa |}) pa').
-        unfold cache_hit.
-        rewrite <- add_2; [| exact Hneqi ].
-        rewrite Heqa' in Hcache_hit.
-        simpl in Hcache_hit.
-        unfold cache_hit, global_update_in_cache in Hcache_hit.
-        destruct (cache_hit_dec (cache ax) pa) as [Hcache_hit_x_pa|Hncache_hit_x_pa].
-        unfold update_in_cache in Hcache_hit.
-        rewrite <- add_2 in Hcache_hit; [| exact Hneqi ].
-        exact Hcache_hit.
-        apply Hncache_hit_x_pa in Hcache_hit_pa.
-        destruct Hcache_hit_pa.
-        destruct (cache_hit_dec
-                    (add_in_map (cache ax) (phys_to_index pa)
-                                {| dirty := true; content := c'; tag := pa |}) pa') as [Hcache_add|Hncache_add].
-        rewrite <- add_2.
-        unfold cache_clean_inv in Hclean.
-        destruct H as [Hsmramcx [Hsmramx [Hsmrrx [Hcleanx Hipx]]]].
-        assert (cache_hit (cache ax) pa') as Hcache_hit_x_pa'; [
-            apply (cache_hit_is_preserve_by_non_conflicted_update (cache ax)
-                                                                  (cache a')
-                                                                  pa
-                                                                  pa'
-                                                                  c'); [
-            exact Hneqi |
-            rewrite Heqa'; simpl; reflexivity |
-            exact Hcache_hit ] |].
-        assert (find_cache_content ax pa' = Some (content (find_in_map (cache ax) (phys_to_index pa')))) as Hfind.
-        unfold find_cache_content, find_in_cache.
-        destruct (cache_hit_dec (cache ax) pa') as [_H|_H]; [ reflexivity | intuition ].
-        rewrite <- Hfind.
-        apply (Hcleanx pa' Hinside' Hcache_hit_x_pa').
-        exact Hneqi.
-        apply Hncache_add in H0.
-        destruct H0.
-    * destruct (eq_dec (phys_to_index pa) (phys_to_index pa')) as [Heqi|Hneqi].
-      - assert (cache a'=global_update_in_cache (cache ax) pa c') as Heqcache'; [
-          rewrite Heqa';
-          simpl;
-          reflexivity |].
-        assert (cache_hit (global_update_in_cache (cache ax) pa c') pa); [
-            apply (global_update_in_cache_cache_hit (cache ax) pa) |].
-        rewrite <- Heqcache' in H0.
-        destruct (eq_dec pa pa') as [Heq|Hneq].
-        (* case addr_eq *)
-        apply eq_equal in Heq.
-        rewrite Heq in Heqc'.
-        unfold smram_code_inv in Hsmram.
-        assert (is_inside_smram pa'); try exact Hinside'.
-        rewrite <- Heq in Hinside'.
-        apply Hin_smm in Hinside'.
-        unfold is_in_smm in Hinside'.
-        unfold phys_to_hard, translate_physical_address in Heqc'.
-        rewrite <- Heq in Heqc'.
-        destruct (is_inside_smram_dec pa).
-        rewrite Hinside' in Heqc'.
-        destruct (can_access_smram_dec (memory_controller a) true).
-        rewrite Hsmram in Heqc'; try trivial.
-        rewrite Heqc'.
-        unfold find_in_cache, load_in_cache.
-        rewrite <- Heq.
-        destruct cache_hit_dec.
-        rewrite add_1.
-        simpl.
-        reflexivity.
-        unfold cache_hit in n.
-        rewrite add_1 in n.
-        simpl in n.
-        unfold not in n.
-        assert (eq pa pa) by (apply eq_refl).
-        apply n in H2.
-        destruct H2.
-        unfold can_access_smram in n.
-        apply not_or_and in n.
-        destruct n as [G1 G2].
-        intuition.
-        rewrite <- Heq in H1.
-        intuition.
-        (* case ~ addr_eq *)
-        apply (global_update_not_cache_hit (cache ax) (cache a') pa pa' c') in Heqcache'; try intuition.
-      - unfold find_in_cache, load_in_cache.
-        destruct cache_hit_dec.
-        rewrite <- add_2.
-        destruct H as [Hsmramcx [Hsmramx [Hsmrrx [Hcleanx Hipx]]]].
-        assert (cache_hit (cache ax) pa') as Hcache_hit_before; [
-            apply (cache_hit_is_preserve_by_non_conflicted_update (cache ax)
-                                                                  (cache a')
-                                                                  pa
-                                                                  pa'
-                                                                  c'); [
-              exact Hneqi
-            | rewrite Heqa'; reflexivity
-            | exact Hcache_hit ] |].
-        unfold cache_clean_inv in Hcleanx.
-        assert ((if cache_hit_dec (cache ax) pa'
-                 then Some (content (find_in_map (cache ax) (phys_to_index pa')))
-                 else None) = Some smm).
-        apply (Hcleanx _ Hinside' Hcache_hit_before).
-        destruct cache_hit_dec; [ | intuition ].
-        rewrite H.
-        reflexivity.
-        exact Hneqi.
-        destruct H as [Hsmramcx [Hsmramx [Hsmrrx Hcleanx]]].
-        assert (cache_hit (cache ax) pa') as Hcache_hit_before; [
-            apply (cache_hit_is_preserve_by_non_conflicted_update (cache ax) (cache a') pa pa' c'); [
-              exact Hneqi
-            | rewrite Heqa'; reflexivity
-            | exact Hcache_hit ] |].
-        exfalso.
-        apply n.
-        unfold cache_hit.
-        rewrite <- add_2.
-        exact Hcache_hit_before.
-        exact Hneqi.
-  + unfold cache_clean_inv.
-    intros pa' Hinside' Hcache_hit'.
-    remember (find_memory_content a (phys_to_hard a pa)) as c.
-    unfold phys_to_hard, translate_physical_address in Heqc.
-    destruct is_inside_smram_dec.
-    * assert (is_in_smm (proc a)).
-      apply Hin_smm.
-      exact i.
-      assert (can_access_smram (memory_controller a) (in_smm (proc a))).
-      unfold can_access_smram.
-      left.
-      exact H.
-      destruct can_access_smram_dec; [| intuition ].
-      rewrite Hsmram in Heqc ; [| exact i ].
-      rewrite Heqc in Heqa'.
-      unfold update_cache_content in Heqa'.
-      remember (global_update_in_cache (cache a) pa smm) as cache'.
-      unfold global_update_in_cache in Heqcache'.
-      destruct (cache_hit_dec (cache a) pa).
-      rewrite Heqa'; rewrite Heqcache'.
-      unfold find_cache_content, find_in_cache, update_cache_content, update_in_cache.
-      simpl.
-      destruct (eq_dec pa pa') as [eq|neq].
-      apply eq_equal in eq.
-      rewrite eq.
-      assert (cache_hit
-                (add_in_map (cache a) (phys_to_index pa')
-                                      {| dirty := true; content := smm; tag := pa' |}) pa').
-      unfold cache_hit.
-      rewrite add_1.
-      apply eq_refl.
-      destruct cache_hit_dec; [| intuition ].
-      rewrite add_1; reflexivity.
-      remember (add_in_map (cache a)
-                                     (phys_to_index pa)
-                                     {| dirty := true; content := smm; tag := pa |}) as cachex.
-      assert (cachex = cache'); [ rewrite Heqcache';
-                                  rewrite Heqcachex;
-                                  reflexivity |].
-      rewrite H1 in *.
-      assert (cache' = cache a').
-      rewrite Heqa'; rewrite Heqcache'; reflexivity.
-      rewrite H2.
-      destruct (cache_hit_dec (cache a') pa') as [Hcache_hit_pa'|_H]; [| try intuition ].
-      destruct (eq_dec (phys_to_index pa) (phys_to_index pa')) as [Heqi|Hneqi].
-      assert (~ cache_hit (cache a') pa'); [| try intuition ].
-      rewrite Heqa'.
-      rewrite Heqcache'.
-      simpl.
-      unfold cache_hit, update_in_cache.
-      apply eq_equal in Heqi.
-      rewrite <- Heqi.
-      rewrite add_1.
-      intro Hnot.
-      apply eq_sym in Hnot.
-      apply neq in Hnot.
-      exact Hnot.
-      rewrite Heqa'.
-      rewrite Heqcache'.
-      simpl.
-      unfold cache_hit, update_in_cache.
-      rewrite <- add_2 with (k:=phys_to_index pa)
-                            (v:={| dirty := true; content := smm; tag := pa |}); [
-        | exact Hneqi].
-      unfold cache_clean_inv in Hclean.
-      assert (cache_hit (cache a) pa').
-      (**********************)
-      rewrite <- H2 in Hcache_hit_pa'.
-      rewrite Heqcache' in Hcache_hit_pa'.
-      unfold update_in_cache in Hcache_hit_pa'.
-      unfold cache_hit in Hcache_hit_pa'.
-      rewrite <- add_2 in Hcache_hit_pa'; [| exact Hneqi ].
-      exact Hcache_hit_pa'.
-      (**********************)
-      assert (find_cache_content a pa' = Some (content (find_in_map (cache a) (phys_to_index pa')))).
-      unfold find_cache_content.
-      unfold find_in_cache.
-      destruct (cache_hit_dec (cache a) pa') as [_H|_H]; [ | try intuition ].
-      reflexivity.
-      rewrite <- H4.
-      rewrite Hclean; [
-          reflexivity
-        | exact Hinside'
-        | exact H3 ].
-      rewrite Heqa'; rewrite Heqcache'.
-      unfold find_cache_content, find_in_cache, load_in_cache, update_in_cache.
-      destruct (eq_dec pa pa') as [Heq|Hneq].
-      apply eq_equal in Heq.
-      rewrite Heq.
-      assert (cache_hit
-                (add_in_map (cache a) (phys_to_index pa')
-                                      {| dirty := false; content := smm; tag := pa' |}) pa').
-      unfold cache_hit.
-      rewrite add_1.
-      apply eq_refl.
-      destruct cache_hit_dec; [| intuition ].
-      simpl.
-      rewrite add_1; reflexivity.
-      remember (add_in_map (cache a)
-                                     (phys_to_index pa)
-                                     {| dirty := false; content := smm; tag := pa |}) as cachex.
-      assert (cachex = cache'); [ rewrite Heqcache';
-                                  rewrite Heqcachex;
-                                  reflexivity |].
-      rewrite H1 in *.
-      assert (cache' = cache a').
-      rewrite Heqa'; rewrite Heqcache'; reflexivity.
-      rewrite H2.
-      destruct (cache_hit_dec (cache a') pa') as [Hcache_hit_pa'|_H]; [| try intuition ].
-      destruct (eq_dec (phys_to_index pa) (phys_to_index pa')) as [Heqi|Hneqi].
-      assert (~ cache_hit (cache a') pa').
-      rewrite Heqa'.
-      rewrite Heqcache'.
-      simpl.
-      unfold cache_hit, load_in_cache.
-      apply eq_equal in Heqi.
-      rewrite <- Heqi.
-      rewrite add_1.
-      intro Hnot.
-      apply eq_sym in Hnot.
-      apply Hneq in Hnot.
-      exact Hnot.
-      simpl.
-      destruct (cache_hit_dec (cache a') pa') as [_H|_H]; intuition.
-      simpl.
-      destruct (cache_hit_dec (cache a') pa') as [_H|_H]; intuition.
-      rewrite  Heqa'.
-      rewrite Heqcachex.
-      simpl.
-      rewrite <- add_2 with (k:=phys_to_index pa)
-                            (v:={| dirty := false; content := smm; tag := pa |}); [
-        | exact Hneqi ].
-      unfold cache_clean_inv in Hclean.
-      assert (cache_hit (cache a) pa') as Hcache_hit_in_a_pa'.
-      (**********************)
-      rewrite <- H2 in Hcache_hit_pa'.
-      rewrite Heqcache' in Hcache_hit_pa'.
-      unfold load_in_cache in Hcache_hit_pa'.
-      unfold cache_hit in Hcache_hit_pa'.
-      rewrite <- add_2 in Hcache_hit_pa'; [| exact Hneqi ].
-      exact Hcache_hit_pa'.
-      (**********************)
-      assert (find_cache_content a pa' = Some (content (find_in_map (cache a) (phys_to_index pa')))) as Hfind.
-      unfold find_cache_content.
-      unfold find_in_cache.
-      destruct (cache_hit_dec (cache a) pa'); [ | try intuition ].
-      reflexivity.
-      rewrite <- Hfind.
-      rewrite Hclean; [
-          reflexivity
-        | exact Hinside'
-        | exact Hcache_hit_in_a_pa' ].
-    * assert (~ eq pa pa'); [
-        apply or_not_and;
-        left;
-        apply (x1_not_in_interval_x2_in_interval_x1_neq_x2 _ _ _ n Hinside') |].
-      destruct (eq_dec (phys_to_index pa) (phys_to_index pa')) as [Heqi|Hneqi].
-      - assert (~ cache_hit (cache a') pa') as Hncache_hit_pa'; [| intuition ].
-        rewrite Heqa'.
-        unfold update_cache_content, cache_hit, global_update_in_cache; simpl.
-        destruct (cache_hit_dec (cache a) pa).
-        unfold update_in_cache.
-        apply eq_equal in Heqi.
-        rewrite <- Heqi.
-        rewrite add_1.
-        simpl.
-        intro Hnot.
-        apply addr_eq_sym in Hnot.
-        apply H in Hnot.
-        exact Hnot.
-        unfold load_in_cache.
-        apply eq_equal in Heqi.
-        rewrite <- Heqi.
-        rewrite add_1.
-        simpl.
-        intro Hnot.
-        apply addr_eq_sym in Hnot.
-        apply H in Hnot.
-        exact Hnot.
-      - assert (cache_hit (cache a) pa').
-        rewrite Heqa' in Hcache_hit'.
-        unfold cache_hit, update_cache_content in Hcache_hit'.
-        simpl in Hcache_hit'.
-        unfold global_update_in_cache in Hcache_hit'.
-        destruct (cache_hit_dec (cache a) pa) as [_H|_H]; [
-            unfold update_in_cache in Hcache_hit';
-            rewrite <- add_2 in Hcache_hit'; [| exact Hneqi ];
-            exact Hcache_hit' |
-            unfold load_in_cache in Hcache_hit' ;
-              rewrite <- add_2 in Hcache_hit'; [| exact Hneqi ] ;
-              exact Hcache_hit' ].
-        assert (find_cache_content a' pa' = find_cache_content a pa').
-        unfold find_cache_content.
-        unfold find_in_cache.
-        do 2 (destruct cache_hit_dec; [| intuition ]).
-        rewrite Heqa'.
-        unfold update_cache_content, global_update_in_cache, load_in_cache, update_in_cache; simpl.
-        destruct cache_hit_dec;
-          (rewrite <- add_2; [ reflexivity | exact Hneqi ]).
-        rewrite H1.
-        rewrite Hclean; [
-            reflexivity
-          | exact Hinside'
-          | exact H0 ].
+    apply (update_cache_with_memory_cache_clean_inv ax a' pa Hinvx);
+      destruct Hinvx as [Hsmramcx [Hsmramx [Hsmrrx [Hcleanx [Hipx Hsmbasex]]]]].
+    - apply update_memory_changes_only_memory in Heqax.
+      destruct Heqax as [_Hmc [Hproc _Hcache]].
+      rewrite <- Hproc.
+      exact Hin_smm.
+    - exact Heqa'.
+  + apply (update_cache_with_memory_cache_clean_inv a a' pa Hinv Hin_smm Heqa').
 Qed.
 
-Lemma load_in_cache_from_memory_preserves_smrr_inv:
-  forall a a' :Architecture Software,
-  forall pa   :PhysicalAddress,
-    inv a
-    -> (is_inside_smram pa -> is_in_smm (proc a))
-    -> a' = load_in_cache_from_memory a pa
-    -> smrr_inv a'.
+Lemma load_in_cache_from_memory_preserves_smrr_inv
+      (a a':    Architecture Software)
+      (pa:      PhysicalAddress)
+      (Hinv:    inv a)
+      (Hin_smm: is_inside_smram pa -> is_in_smm (proc a))
+      (Heqa':   a' = load_in_cache_from_memory a pa)
+  : smrr_inv a'.
 Proof.
-  intros a a' pa [Hsmramc [Hsmram [Hsmrr [Hclean [Hip Hsmbase]]]]] Hin_smm Heqa'.
+  destruct Hinv as [Hsmramc [Hsmram [Hsmrr [Hclean [Hip Hsmbase]]]]].
   apply load_in_cache_from_memory_changes_only_mem_and_cache in Heqa' as [Hproc Hother].
   unfold smrr_inv.
   rewrite <- Hproc.
   exact Hsmrr.
 Qed.
 
-Lemma load_in_cache_from_memory_preserves_smramc_inv:
-  forall a a' :Architecture Software,
-  forall pa   :PhysicalAddress,
-    inv a
-    -> (is_inside_smram pa -> is_in_smm (proc a))
-    -> a' = load_in_cache_from_memory a pa
-    -> smramc_inv a'.
+Lemma load_in_cache_from_memory_preserves_smramc_inv
+      (a a':    Architecture Software)
+      (pa:      PhysicalAddress)
+      (Hinv:    inv a)
+      (Hin_smm: is_inside_smram pa -> is_in_smm (proc a))
+      (Heqa':   a' = load_in_cache_from_memory a pa)
+  : smramc_inv a'.
 Proof.
-  intros a a' pa [Hsmramc [Hsmram [Hsmrr [Hclean [Hip Hsmbase]]]]] Hin_smm Heqa'.
+  destruct Hinv as [Hsmramc [Hsmram [Hsmrr [Hclean [Hip Hsmbase]]]]].
   apply load_in_cache_from_memory_changes_only_mem_and_cache in Heqa' as [Hproc Hother].
   unfold smramc_inv.
   rewrite <- Hother.
   exact Hsmramc.
 Qed.
 
-Lemma load_in_cache_from_memory_preserves_smbase_inv:
-  forall a a' :Architecture Software,
-  forall pa   :PhysicalAddress,
-    inv a
-    -> (is_inside_smram pa -> is_in_smm (proc a))
-    -> a' = load_in_cache_from_memory a pa
-    -> smbase_inv a'.
+Lemma load_in_cache_from_memory_preserves_smbase_inv
+      (a a':    Architecture Software)
+      (pa:      PhysicalAddress)
+      (Hinv:    inv a)
+      (Hin_smm: is_inside_smram pa -> is_in_smm (proc a))
+      (Heqa':   a' = load_in_cache_from_memory a pa)
+  : smbase_inv a'.
 Proof.
-  intros a a' pa [Hsmramc [Hsmram [Hsmrr [Hclean [Hip Hsmbase]]]]] Hin_smm Heqa'.
+  destruct Hinv as [Hsmramc [Hsmram [Hsmrr [Hclean [Hip Hsmbase]]]]].
   apply load_in_cache_from_memory_changes_only_mem_and_cache in Heqa' as [Hproc Hother].
   unfold smbase_inv.
   rewrite <- Hproc.
   exact Hsmbase.
 Qed.
 
-Lemma load_in_cache_from_memory_preserves_ip_inv:
-  forall a a' :Architecture Software,
-  forall pa   :PhysicalAddress,
-    inv a
-    -> (is_inside_smram pa -> is_in_smm (proc a))
-    -> a' = load_in_cache_from_memory a pa
-    -> ip_inv a'.
+Lemma load_in_cache_from_memory_preserves_ip_inv
+      (a a':    Architecture Software)
+      (pa:      PhysicalAddress)
+      (Hinv:    inv a)
+      (Hin_smm: is_inside_smram pa -> is_in_smm (proc a))
+      (Heqa':   a' = load_in_cache_from_memory a pa)
+  : ip_inv a'.
 Proof.
-  intros a a' pa [Hsmramc [Hsmram [Hsmrr [Hclean [Hip Hsmbase]]]]] Hin_smm Heqa'.
+  destruct Hinv as [Hsmramc [Hsmram [Hsmrr [Hclean [Hip Hsmbase]]]]].
   apply load_in_cache_from_memory_changes_only_mem_and_cache in Heqa' as [Hproc Hother].
   unfold ip_inv.
   rewrite <- Hproc.
@@ -902,15 +723,14 @@ Proof.
   exact Hip.
 Qed.
 
-Lemma load_in_cache_from_memory_preserves_inv:
-  forall a a' :Architecture Software,
-  forall pa   :PhysicalAddress,
-    inv a -> (is_inside_smram pa -> is_in_smm (proc a))
-    -> a' = load_in_cache_from_memory a pa
-    -> inv a'.
+Lemma load_in_cache_from_memory_preserves_inv
+      (a a':    Architecture Software)
+      (pa:      PhysicalAddress)
+      (Hinv:    inv a)
+      (Hin_smm: is_inside_smram pa -> is_in_smm (proc a))
+      (Heqa':   a' = load_in_cache_from_memory a pa)
+  : inv a'.
 Proof.
-  intros a a' pa.
-  intros Hinv Hsmm Heqa'.
   unfold inv.
   split; [| split; [| split; [| split; [| split]]]]; [
       eapply (load_in_cache_from_memory_preserves_smramc_inv a a' pa)
@@ -921,42 +741,48 @@ Proof.
     | eapply (load_in_cache_from_memory_preserves_smbase_inv a a' pa) ]; trivial.
 Qed.
 
-Lemma update_cache_content_with_context_preserves_smramc_inv:
-  forall a a' :Architecture Software,
-  forall pa   :PhysicalAddress,
-    inv a -> (is_inside_smram pa -> is_in_smm (proc a))
-    -> a' = update_cache_content a pa (smm_context a)
-    -> smramc_inv a'.
+Lemma update_cache_content_with_context_preserves_smramc_inv
+      (a a':    Architecture Software)
+      (pa:      PhysicalAddress)
+      (val:     Value)
+      (Hinv:    inv a)
+      (Hin_smm: is_inside_smram pa -> is_in_smm (proc a))
+      (Heqa':   a' = update_cache_content a pa (val, (smm_context a)))
+  : smramc_inv a'.
 Proof.
-  intros a a' pa [Hsmramc [Hsmram [Hsmrr [Hclean [Hip Hsmbase]]]]] Hin_smm Heqa'.
+  destruct Hinv as [Hsmramc [Hsmram [Hsmrr [Hclean [Hip Hsmbase]]]]].
   apply update_cache_changes_only_cache in Heqa' as [Hproc [Hmc Hother]].
   unfold smramc_inv.
   rewrite <- Hmc.
   exact Hsmramc.
 Qed.
 
-Lemma update_cache_content_with_context_preserves_smrr_inv:
-  forall a a' :Architecture Software,
-  forall pa   :PhysicalAddress,
-    inv a -> (is_inside_smram pa -> is_in_smm (proc a))
-    -> a' = update_cache_content a pa (smm_context a)
-    -> smrr_inv a'.
+Lemma update_cache_content_with_context_preserves_smrr_inv
+      (a a':    Architecture Software)
+      (pa:      PhysicalAddress)
+      (val:     Value)
+      (Hinv:    inv a)
+      (Hin_smm: is_inside_smram pa -> is_in_smm (proc a))
+      (Heqa':   a' = update_cache_content a pa (val, (smm_context a)))
+  : smrr_inv a'.
 Proof.
-  intros a a' pa [Hsmramc [Hsmram [Hsmrr [Hclean Hsmbase]]]] Hin_smm Heqa'.
+  destruct Hinv as [Hsmramc [Hsmram [Hsmrr [Hclean [Hip Hsmbase]]]]].
   apply update_cache_changes_only_cache in Heqa' as [Hproc [Hmc Hother]].
   unfold smrr_inv.
   rewrite <- Hproc.
   exact Hsmrr.
 Qed.
 
-Lemma update_cache_content_with_context_preserves_smram_code_inv:
-  forall a a' :Architecture Software,
-  forall pa   :PhysicalAddress,
-    inv a -> (is_inside_smram pa -> is_in_smm (proc a))
-    -> a' = update_cache_content a pa (smm_context a)
-    -> smram_code_inv a'.
+Lemma update_cache_content_with_context_preserves_smram_code_inv
+      (a a':    Architecture Software)
+      (pa:      PhysicalAddress)
+      (val:     Value)
+      (Hinv:    inv a)
+      (Hin_smm: is_inside_smram pa -> is_in_smm (proc a))
+      (Heqa':   a' = update_cache_content a pa (val, (smm_context a)))
+  : smram_code_inv a'.
 Proof.
-  intros a a' pa [Hsmramc [Hsmram [Hsmrr [Hclean [Hip Hsmbase]]]]] Hin_smm Heqa'.
+  destruct Hinv as [Hsmramc [Hsmram [Hsmrr [Hclean [Hip Hsmbase]]]]].
   apply update_cache_changes_only_cache in Heqa' as [Hproc [Hmc Hmem]].
   unfold smram_code_inv.
   unfold find_memory_content.
@@ -964,14 +790,16 @@ Proof.
   exact Hsmram.
 Qed.
 
-Lemma update_cache_content_with_context_preserves_ip_inv:
-  forall a a' :Architecture Software,
-  forall pa   :PhysicalAddress,
-    inv a -> (is_inside_smram pa -> is_in_smm (proc a))
-    -> a' = update_cache_content a pa (smm_context a)
-    -> ip_inv a'.
+Lemma update_cache_content_with_context_preserves_ip_inv
+      (a a':    Architecture Software)
+      (pa:      PhysicalAddress)
+      (val:     Value)
+      (Hinv:    inv a)
+      (Hin_smm: is_inside_smram pa -> is_in_smm (proc a))
+      (Heqa':   a' = update_cache_content a pa (val, (smm_context a)))
+  : ip_inv a'.
 Proof.
-  intros a a' pa [Hsmramc [Hsmram [Hsmrr [Hclean [Hip Hsmbase]]]]] Hin_smm Heqa'.
+  destruct Hinv as [Hsmramc [Hsmram [Hsmrr [Hclean [Hip Hsmbase]]]]].
   apply update_cache_changes_only_cache in Heqa' as [Hproc [Hmc Hmem]].
   unfold ip_inv.
   rewrite <- Hproc.
@@ -979,43 +807,54 @@ Proof.
   exact Hip.
 Qed.
 
-Lemma update_cache_content_with_context_preserves_smbase_inv:
-  forall a a' :Architecture Software,
-  forall pa   :PhysicalAddress,
-    inv a -> (is_inside_smram pa -> is_in_smm (proc a))
-    -> a' = update_cache_content a pa (smm_context a)
-    -> smbase_inv a'.
+Lemma update_cache_content_with_context_preserves_smbase_inv
+      (a a':    Architecture Software)
+      (pa:      PhysicalAddress)
+      (val:     Value)
+      (Hinv:    inv a)
+      (Hin_smm: is_inside_smram pa -> is_in_smm (proc a))
+      (Heqa':   a' = update_cache_content a pa (val, (smm_context a)))
+  : smbase_inv a'.
 Proof.
-  intros a a' pa [Hsmramc [Hsmram [Hsmrr [Hclean [Hip Hsmbase]]]]] Hin_smm Heqa'.
+  destruct Hinv as [Hsmramc [Hsmram [Hsmrr [Hclean [Hip Hsmbase]]]]].
   apply update_cache_changes_only_cache in Heqa' as [Hproc [Hmc Hmem]].
   unfold smbase_inv.
   rewrite <- Hproc.
   exact Hsmbase.
 Qed.
 
-Lemma update_cache_content_with_context_preserves_cache_clean_inv:
-  forall a a' :Architecture Software,
-  forall pa   :PhysicalAddress,
-    inv a -> (is_inside_smram pa -> is_in_smm (proc a))
-    -> a' = update_cache_content a pa (smm_context a)
-    -> cache_clean_inv a'.
+Lemma update_cache_content_with_context_preserves_cache_clean_inv
+      (a a':    Architecture Software)
+      (pa:      PhysicalAddress)
+      (val:     Value)
+      (Hinv:    inv a)
+      (Hin_smm: is_inside_smram pa -> is_in_smm (proc a))
+      (Heqa':   a' = update_cache_content a pa (val, (smm_context a)))
+  : cache_clean_inv a'.
 Proof.
-  intros a a' pa [Hsmramc [Hsmram [Hsmrr [Hclean [Hip Hsmbase]]]]] Hin_smm Heqa'.
+  destruct Hinv as [Hsmramc [Hsmram [Hsmrr [Hclean [Hip Hsmbase]]]]].
   unfold cache_clean_inv.
-  intros pa' Hinside' Hcache_hit'.
-  unfold update_cache_content in Heqa'.
-  unfold global_update_in_cache in Heqa'.
+  intros pa' val' s' Hinside' Hcache_hit' Hfind'.
+  assert (cache a' = global_update_in_cache (cache a) pa (val, smm_context a))
+    as Heqcache
+      by (rewrite Heqa'; reflexivity).
+  unfold global_update_in_cache in Heqcache.
   destruct (cache_hit_dec (cache a) pa).
-  + unfold update_in_cache in Heqa'.
-    unfold find_cache_content.
-    unfold find_in_cache.
+  + unfold update_in_cache in Heqcache.
+    unfold find_cache_content in Hfind'.
+    unfold find_in_cache in Hfind'.
     destruct cache_hit_dec; [| intuition ].
-    rewrite Heqa'; simpl.
+    rewrite Heqa' in Hfind'; simpl.
     destruct (eq_dec pa pa') as [Heq|Hneq].
     * apply eq_equal in Heq.
-      rewrite <- Heq.
-      rewrite add_1.
-      simpl.
+      rewrite <- Heq in Hfind'.
+      unfold update_cache_content, global_update_in_cache in Hfind'.
+      simpl in Hfind'.
+      destruct cache_hit_dec; [| intuition ].
+      unfold update_in_cache in Hfind'.
+      rewrite add_1 in Hfind'.
+      simpl in Hfind'.
+      inversion Hfind'.
       rewrite <- Heq in Hinside'.
       apply Hin_smm in Hinside'.
       unfold smm_context.
@@ -1028,124 +867,125 @@ Proof.
         assert (cache_hit (cache a') pa) as Hcache_hit_pa.
         unfold cache_hit.
         rewrite Heqa'.
+        unfold update_cache_content, global_update_in_cache, update_in_cache.
         simpl.
+        destruct cache_hit_dec; [| intuition ].
         rewrite add_1.
         simpl.
         apply addr_eq_refl.
         apply (cache_hit_same_index_cache_miss (cache a') pa pa' Hcache_hit_pa Hneq Heqi).
-      - rewrite <- add_2; [| exact Hneqi ].
+      - simpl in Hfind'.
+        unfold global_update_in_cache, update_in_cache in Hfind'.
+        destruct cache_hit_dec; [| intuition].
+        rewrite <- add_2 in Hfind' ; [| exact Hneqi ].
         assert (cache_hit (cache a) pa').
         apply (cache_hit_is_preserve_by_non_conflicted_update (cache a)
                                                               (cache a')
                                                               pa pa'
-                                                              (smm_context a)
+                                                              (val, smm_context a)
                                                               Hneqi).
         rewrite Heqa'.
         simpl.
-        unfold global_update_in_cache.
-        destruct cache_hit_dec as [_H|Hncache_hit] ; [
-          unfold update_in_cache;
-          reflexivity
-        | apply Hncache_hit in c;
-          destruct c;
-          exact c0 ].
+        reflexivity.
         exact Hcache_hit'.
-        assert (find_cache_content a pa' = Some (content (find_in_map (cache a) (phys_to_index pa')))) as Hfind.
+        inversion Hfind'.
+        unfold cache_clean_inv in Hclean.
+        apply (Hclean pa' val' s' Hinside' H).
         unfold find_cache_content, find_in_cache.
-        destruct cache_hit_dec as [_H|Hncache_hit]; [ reflexivity |].
-        apply Hncache_hit in H; destruct H.
-        rewrite <- Hfind.
-        rewrite Hclean; [
-            reflexivity |
-            exact Hinside' |
-            exact H ].
-  + unfold load_in_cache in Heqa'.
-    unfold find_cache_content.
-    unfold find_in_cache.
+        destruct cache_hit_dec; [| intuition].
+        rewrite H1.
+        reflexivity.
+  + unfold load_in_cache in Heqcache.
+    unfold find_cache_content in Hfind'.
+    unfold find_in_cache in Hfind'.
     destruct cache_hit_dec; [| intuition ].
-    rewrite Heqa'; simpl.
+    rewrite Heqa' in Hfind'; simpl in Hfind'.
+    inversion Hfind'.
     destruct (eq_dec pa pa') as [Heqpa|Hneqpa].
     * apply eq_equal in Heqpa.
-      rewrite <- Heqpa.
-      rewrite add_1.
-      simpl.
+      rewrite <- Heqpa in H0.
+      unfold global_update_in_cache in H0.
+      destruct cache_hit_dec; [intuition|].
+      unfold load_in_cache in H0.
+      rewrite add_1 in H0.
+      simpl in H0.
+      inversion H0.
       rewrite <- Heqpa in Hinside'.
       apply Hin_smm in Hinside'.
       unfold smm_context.
       destruct is_in_smm_dec.
       reflexivity.
-      apply n0 in Hinside'.
+      apply n1 in Hinside'.
       destruct Hinside'.
     * destruct (eq_dec (phys_to_index pa) (phys_to_index pa')) as [Heqi|Hneqi].
       - assert (~ cache_hit (cache a') pa'); [| intuition ].
         assert (cache_hit (cache a') pa).
         unfold cache_hit.
         rewrite Heqa'.
+        unfold update_cache_content, global_update_in_cache, load_in_cache.
         simpl.
+        destruct cache_hit_dec; [intuition|].
         rewrite add_1.
         simpl.
         apply addr_eq_refl.
         apply (cache_hit_same_index_cache_miss (cache a') pa pa' H Hneqpa Heqi).
-      - rewrite <- add_2; [| exact Hneqi ].
+      - unfold update_cache_content, global_update_in_cache, load_in_cache in H0.
+        destruct cache_hit_dec; [intuition|].
+        rewrite <- add_2 in H0; [| exact Hneqi ].
         assert (cache_hit (cache a) pa').
         apply (cache_hit_is_preserve_by_non_conflicted_update (cache a)
                                                               (cache a')
                                                               pa pa'
-                                                              (smm_context a)
+                                                              (val, smm_context a)
                                                               Hneqi).
         rewrite Heqa'.
         simpl.
-        unfold global_update_in_cache.
-        destruct cache_hit_dec; [ intuition |].
-        unfold load_in_cache.
         reflexivity.
-        exact c.
-        assert (find_cache_content a pa' = Some (content (find_in_map (cache a) (phys_to_index pa')))).
+        exact Hcache_hit'.
+        unfold cache_clean_inv in Hclean.
+        apply (Hclean pa' val' s' Hinside' H).
         unfold find_cache_content, find_in_cache.
-        destruct cache_hit_dec.
+        destruct cache_hit_dec; [|intuition].
+        rewrite H0.
         reflexivity.
-        apply n0 in H; destruct H.
-        rewrite <- H0.
-        rewrite Hclean; [
-            reflexivity |
-            exact Hinside' |
-            exact H ].
 Qed.
 
-Lemma update_cache_content_with_context_preserves_inv:
-  forall a a' :Architecture Software,
-  forall pa   :PhysicalAddress,
-    inv a -> (is_inside_smram pa -> is_in_smm (proc a))
-    -> a' = update_cache_content a pa (smm_context a)
-    -> inv a'.
+Lemma update_cache_content_with_context_preserves_inv
+      (a a':    Architecture Software)
+      (pa:      PhysicalAddress)
+      (val:     Value)
+      (Hinv:    inv a)
+      (Hin_smm: is_inside_smram pa -> is_in_smm (proc a))
+      (Heqa':   a' = update_cache_content a pa (val, (smm_context a)))
+  : inv a'.
 Proof.
-  intros a a' pa.
-  intros Hinv Hsmm Heqa'.
   unfold inv.
   split; [| split; [| split; [| split; [| split]]]]; [
-      eapply (update_cache_content_with_context_preserves_smramc_inv a a' pa)
-    | eapply (update_cache_content_with_context_preserves_smram_code_inv a a' pa)
-    | eapply (update_cache_content_with_context_preserves_smrr_inv a a' pa)
-    | eapply (update_cache_content_with_context_preserves_cache_clean_inv a a' pa)
-    | eapply (update_cache_content_with_context_preserves_ip_inv a a' pa)
-    | eapply (update_cache_content_with_context_preserves_smbase_inv a a' pa) ]; trivial.
+      eapply (update_cache_content_with_context_preserves_smramc_inv a a' pa val)
+    | eapply (update_cache_content_with_context_preserves_smram_code_inv a a' pa val)
+    | eapply (update_cache_content_with_context_preserves_smrr_inv a a' pa val)
+    | eapply (update_cache_content_with_context_preserves_cache_clean_inv a a' pa val)
+    | eapply (update_cache_content_with_context_preserves_ip_inv a a' pa val)
+    | eapply (update_cache_content_with_context_preserves_smbase_inv a a' pa val) ]; trivial.
 Qed.
 
-Lemma load_then_update_cache_with_context_preserves_inv:
-  forall a a' :Architecture Software,
-  forall pa   :PhysicalAddress,
-    inv a -> (is_inside_smram pa -> is_in_smm (proc a))
-    -> a' = update_cache_content (load_in_cache_from_memory a pa) pa (smm_context a)
-    -> inv a'.
+Lemma load_then_update_cache_with_context_preserves_inv
+      (a a'':   Architecture Software)
+      (pa:      PhysicalAddress)
+      (val:     Value)
+      (Hinv:    inv a)
+      (Hin_smm: is_inside_smram pa -> is_in_smm (proc a))
+      (Heqa'':  a'' = update_cache_content (load_in_cache_from_memory a pa) pa (val, smm_context a))
+  : inv a''.
 Proof.
-  intros a a'' pa Hinv Hin_smm Heqa''.
   remember (load_in_cache_from_memory a pa) as a'.
-  assert (inv a') as Hinv'.
-  apply (load_in_cache_from_memory_preserves_inv a a' pa Hinv Hin_smm Heqa').
+  assert (inv a')
+    as Hinv'
+      by (apply (load_in_cache_from_memory_preserves_inv a a' pa Hinv Hin_smm Heqa')).
   assert (proc a = proc a').
   apply load_in_cache_from_memory_changes_only_mem_and_cache in Heqa' as [Hproc _H].
   exact Hproc.
   rewrite H in Hin_smm.
   rewrite (context_is_preserves a a' H) in Heqa''.
-  apply (update_cache_content_with_context_preserves_inv a' a'' pa Hinv' Hin_smm Heqa'').
+  apply (update_cache_content_with_context_preserves_inv a' a'' pa val Hinv' Hin_smm Heqa'').
 Qed.
