src/x86/Transition/Event/EnableInterrupt.v
@@ -2,7 +2,7 @@ Require Import SpecCert.x86.Architecture.
 Require Import SpecCert.Address.
 
 Definition enable_interrupt_post
-           {S :Set} :=
-  fun (a a':Architecture S) =>
-    let p' := enable_interrupt (proc a)
-    in a' = update_proc a p'.
+           {Label: Type}
+           (a a':Architecture Label) :=
+  let p' := enable_interrupt (proc a)
+  in a' = update_proc a p'.
