src/x86/Transition/Event/OpenSmram.v
@@ -1,13 +1,12 @@
 Require Import SpecCert.x86.Architecture.
 
 Definition open_smram_pre
-           {S :Set} :=
-  fun (a:Architecture S) =>
-    smramc_is_unlocked (memory_controller a).
+           {Label: Type}
+           (a:     Architecture Label) :=
+  smramc_is_unlocked (memory_controller a).
 
 Definition open_smram_post
-           {S :Set} :=
-  fun (a a':Architecture S) =>
+           {Label: Type}
+           (a a':  Architecture Label) :=
     exists h, let m' := open_smram (memory_controller a) h
     in a' = update_memory_controller a m'.
-
