src/x86/Transition/Event/ReceiveInterrupt.v
@@ -2,8 +2,8 @@ Require Import SpecCert.x86.Architecture.
 Require Import SpecCert.Address.
 
 Definition receive_interrupt_post
-           {S :Set}
-           (i :Interrupt) :=
-  fun (a a':Architecture S) =>
-    let p' := receive_interrupt (proc a) i in
-    a' = update_proc a p'.
+           {Label: Type}
+           (i:     Interrupt)
+           (a a':Architecture Label) :=
+  let p' := receive_interrupt (proc a) i in
+  a' = update_proc a p'.
